src/Lean/Compiler/LCNF/ReduceJpArity.lean
@@ -18,7 +18,7 @@ namespace ReduceJpArity
 
 abbrev ReduceM := ReaderT (FVarIdMap (Array Bool)) CompilerM
 
-partial def reduce (code : Code) : ReduceM Code := do
+partial def reduce (code : Code .pure) : ReduceM (Code .pure) := do
   match code with
   | .let decl k => return code.updateLet! decl (← reduce k)
   | .fun decl k =>
@@ -69,12 +69,14 @@ open ReduceJpArity
 /--
 Try to reduce arity of join points
 -/
-def Decl.reduceJpArity (decl : Decl) : CompilerM Decl := do
+def Decl.reduceJpArity (decl : Decl .pure) : CompilerM (Decl .pure) := do
   let value ← decl.value.mapCodeM reduce |>.run {}
   return { decl with value }
 
-def reduceJpArity (phase := Phase.base) : Pass :=
-  .mkPerDeclaration `reduceJpArity Decl.reduceJpArity phase
+-- TODO: This can be made IRPhase generic
+def reduceJpArity (phase := PassPhase.base) : Pass :=
+  phase.withIRPhaseCheck .pure fun h =>
+    .mkPerDeclaration `reduceJpArity phase (h ▸ Decl.reduceJpArity)
 
 builtin_initialize
   registerTraceClass `Compiler.reduceJpArity (inherited := true)
